\documentclass[a4paper]{article}
\usepackage{amsmath}
\def\npart {IB}
\def\nterm {Michaelmas}
\def\nyear {2017}
\def\nlecturer {?}
\def\ncourse {Methods Example Sheet 1}

\input{header}
\newtheorem*{soln}{Solution}

\renewcommand{\thesection}{}
\renewcommand{\thesubsection}{\arabic{section}.\arabic{subsection}}
\makeatletter
\def\@seccntformat#1{\csname #1ignore\expandafter\endcsname\csname the#1\endcsname\quad}
\let\sectionignore\@gobbletwo
\let\latex@numberline\numberline
\def\numberline#1{\if\relax#1\relax\else\latex@numberline{#1}\fi}
\makeatother


\begin{document}
	
\maketitle

\section{QUESTION 1}

\[ \frac{f(x_{+} + f(x_{-}))}{2} = \frac{1}{2} a_{0} + \sum_{n=1}^{\infty} \left[ a_{n} \cos \left( \frac{n \pi x}{L} \right) + b_{n} \sin \left( \frac{n \pi x}{L} \right)  \right]  \]

For $ f(x) = (x-1)^{2} $ on the interval $ -1 \leq x \leq 1 $, $ f(x) $ is an even function, thus $ b_{n} = 0 $. We have $ L = 1 $, and 

\begin{align*}
\frac{1}{2} a_{0} & = \frac{1}{2L} \int_{-L}^{L} f(x) \; \d x \\
& = \frac{1}{2} \int_{-1}^{1} x^{4} - 2x^{2} + 1 \; \d x \\
& = \int_{0}^{1} x^{4} - 2x^{2} + 1 \; \d x \\
& = \frac{8}{15}
\end{align*}

and

\begin{align*}
a_{n} & = \frac{1}{L} \int_{-1}^{1} f(x) \cos \left( \frac{n \pi x}{L} \right) \; \d x   \\
& = \int_{-1}^{1} x^{4} \cos  n \pi x  \; \d x - 2 \int_{-1}^{1} x^{2} \cos  n \pi x   \; \d x + \int_{-1}^{1} \cos  n \pi x   \; \d x
\end{align*}

Evaluating each integral separately, we have:

\begin{enumerate}
	\item  \[ \int_{-1}^{1} \cos  n \pi x   \; \d x = \left[ \frac{\sin n \pi x}{n \pi} \right]_{-1}^{-1} = 0  \]
	
	as $ \sin n \pi x = 0 \; \forall \; n $
	
	\item By parts, 
	
	\begin{align*}
	\int_{-1}^{1} x^{2} \cos  n \pi x   \; \d x & = \left[ \frac{x^{2} \sin n \pi x}{n \pi} - \frac{1}{n \pi }\int 2x \sin n \pi x \; \d x \right]_{-1}^{1}  \\
	& = - \frac{2}{n \pi} \int_{-1}^{1} x \sin n \pi x \; \d x
	\end{align*}
	
	and
	
	\begin{align*}
	\int_{-1}^{1} x \sin n \pi x \; \d x & = \left[  \frac{- x \cos n \pi x}{n \pi} + \frac{1}{n \pi} \int \cos n \pi x \; \d x   \right]_{-1}^{1}  \\
	& = \frac{-2 \cos n \pi x }{(n \pi )^{2}}
	\end{align*}
	
	Thus the second integral contributes to give
	
	\[ - \frac{8 cos n \pi x}{(n \pi)^{2}} \]
	
	
	\item 
	
	\begin{align*}
	\int_{-1}^{1} x^{4} \cos  n \pi x  \; \d x & = \left[ \frac{x^{4} \sin n \pi x}{n \pi} - \frac{1}{n \pi }\int 4x^{3} \sin n \pi x \; \d x  \right]_{-1}^{1} \\
	& = - \frac{4}{n \pi} \int_{-1}^{1} x^{3} \sin n \pi x \; \d x
	\end{align*}
	
	and 
	
	\begin{align*}
	\int_{-1}^{1} x^{3} \sin n \pi x \; \d x & = \left[ \frac{-x^{3} \cos n \pi x}{n \pi} + \frac{1}{n \pi} \int 3 x^{2} \cos n \pi x \right]_{-1}^{1}  \\
	& = \frac{-2 \cos n \pi}{n \pi} + \frac{3}{n \pi} \int_{-1}^{1} x^{2} \cos n \pi x \; \d x
	\end{align*}
	
	Whence
	
	\begin{align*}
	\int_{-1}^{1} x^{4} \cos  n \pi x  \; \d x & = \frac{8\cos n \pi}{n \pi} - \frac{12}{(n \pi)^{2} } \int_{-1}^{1} x^{2} \cos n \pi x \; \d x  \\
	& = \frac{8\cos n \pi}{n \pi} - \frac{48 \cos n \pi }{(n \pi)^{4}}
	\end{align*}
	
	using (ii).
	
	
	
\end{enumerate}

Finally,

\begin{align*}
a_{n} & = - \frac{48 \cos n \pi }{(n \pi)^{4}} \\
& = \frac{48(-1)^{n+1}}{(n \pi)^{4}}
\end{align*}

as $ \cos n \pi x = (-1)^{n}$ 

Hence the Fourier Series is given by

\begin{align*}
f(x) & = \frac{1}{2}a_{0} + \sum_{n=1}^{\infty} a_{n} \cos n \pi x \\
& = \frac{8}{15} + \frac{48}{\pi^{4}}\sum_{n=1}^{\infty} \frac{(-1)^{n+1}}{n^{4}} \cos n \pi x
\end{align*}

\begin{center}
	\begin{tikzpicture}
	\draw [->] (-5, 0) -- (5, 0) node [right] {$x$};
	\draw [->, use as bounding box] (0, -2.5) -- (0, 2.5) node [above] {$f(x)$};
	
	\end{tikzpicture}
\end{center}


$ f(x) $ satisfies the Dirichlet conditions. The $ 1^{\text{st}} $ derivative is the lowest derivative which is discontinuous (at the endpoints, as $ f(x) $ even fn $ \Rightarrow \; f'(x) $ odd), so Fourier coefficients are $ \Oc(\frac{1}{n^{2}}) $ as $ n \to \infty $

\section{QUESTION 2}

Extending on range $ (-\pi,\pi) $ so $ L = \pi $ and

\begin{enumerate}[label = (\alph*)]
	\item \[ \frac{f(x_{+} + f(x_{-}))}{2} =  \sum_{n=1}^{\infty} b_{n} \sin  n x   \]
	
	where 
	\begin{align*}
	b_{n} & = \frac{2}{L} \int_{0}^{L} f(x) \sin \left( \frac{n \pi x}{L} \right) \; \d x  \\
	& = \frac{2}{\pi} \int_{0}^{\pi} x^{2} \sin n x \; \d x
	\end{align*}
	
	Integrating by parts,
	
	\begin{align*}
	\int_{0}^{\pi} x^{2} \sin n x \; \d x & = \left[  \frac{- x^{2} \cos n x }{n} + \frac{1}{n} \int 2x \cos n x \; \d x \right]_{0}^{\pi}  \\
	& = \frac{- \pi^{2} \cos n \pi}{n} + \frac{2}{n} \int_{0}^{\pi} x \cos n x \; \d x
	\end{align*}
	
	and once again,
	
	\begin{align*}
	\int_{0}^{\pi} x \cos n x \; \d x & =\left[ \frac{x \sin n x}{n} - \frac{1}{n} \int \sin n x \; \d x \right]_{0}^{\pi}  \\
	& = - \frac{1}{n} \int_{0}^{\pi} \sin n x \; \d x \\
	& = - \frac{1}{n} \left[ - \frac{\cos n x}{n} \right]_{0}^{\pi}\\
	& = \frac{1}{n^{2}} (\cos n \pi - 1) 
	\end{align*}
	
	Back substituting in, 
	
	\begin{align*}
	b_{n} & = \frac{2}{\pi} \left( \frac{- \pi^{2} \cos n \pi}{n} + \frac{2}{n^{3}} (\cos n \pi - 1)   \right)  \\
	& = \frac{2}{\pi n^{3}} \left(   - 2 + (2 - (\pi n)^{2} )\cos n \pi       \right) 
	\end{align*}
	
	Hence Fourier sine series given by:
	
	\[ f(x) = \sum_{n=1}^{\infty} \frac{2}{\pi n^{3}} \left(   - 2 + (2 - (\pi n)^{2} ) (-1)^{n} \right) \sin n x  \]
	
	\item Similarly,
	
	\[ \frac{f(x_{+} + f(x_{-}))}{2} =  \frac{a_{0}}{2} + \sum_{n=1}^{\infty} a_{n} \cos n x  \]
	
	where 
	
	\begin{align*}
	\frac{a_{0}}{2} & = \frac{1}{L} \int_{0}^{L} f(x) \; \d x \\
	& = \frac{1}{\pi} \int_{0}^{\pi} x^{2} \; \d x\\
	& = \frac{\pi^{2}}{3}
	\end{align*}
	
	and 
	
	\begin{align*}
	a_{n} & = \frac{2}{L} \int_{0}^{L} f(x) \cos \left( \frac{n \pi x}{L} \right) \; \d x  \\
	& = \frac{2}{\pi} \int_{0}^{\pi} x^{2} \cos n x \; \d x
	\end{align*}
	
	Integrating by parts,
	
	
	\begin{align*}
	\int_{0}^{\pi} x^{2} \cos n x \; \d x & = \left[ \frac{x^{2}\sin n x}{n}  - \frac{1}{n}\int 2x \sin n x \; \d x \right]_{0}^{\pi} \\
	& = \frac{-2}{n} \int_{0}^{\pi} x \sin n x \; \d x
	\end{align*}
	
	and once again,
	
	\begin{align*}
	\int_{0}^{\pi} x \sin n x \; \d x & = \left[  \frac{- x \cos n x}{n} + \frac{1}{n} \int \cos n x \; \d x \right]_{0}^{\pi} \\
	& = \frac{- \pi \cos n \pi}{n} + \frac{1}{n} \left[ \frac{\sin n x}{n \pi} \right]_{0}^{\pi} \\
	& = \frac{- \pi \cos n \pi}{n}
	\end{align*}
	
	Thus
	
	\[ a_{n} = \frac{4}{n^{2}} \cos n \pi  \]
	
	and the Fourier cosine series is given by
	
	\[ f(x) = \frac{\pi^{2}}{3} + \sum_{n=0}^{\infty} \frac{4}{n^{2}} (-1)^{n} \cos n x \]
	
\end{enumerate}

\begin{enumerate}
	\item \begin{center}
		\begin{tikzpicture}
		\draw [->] (-5, 0) -- (5, 0) node [right] {$x$};
		\draw [->, use as bounding box] (0, -2.5) -- (0, 2.5) node [above]
		{$f(x)$};
		\draw node at (-4.5,0) [below] {$ -6 \pi$}; 
		\draw node at (-3,0) [below] {$ -4 \pi$}; 
		\draw node at (-1.5,0) [below] {$ -2 \pi$}; 
		\draw node at (1.5,0) [below] {$ 2 \pi$}; 
		\draw node at (3,0) [below] {$ 4 \pi$}; 
		\draw node at (4.5,0) [below] {$ 6 \pi$}; 
		
		\end{tikzpicture}
	\end{center}
	
	\item \begin{center}
		\begin{tikzpicture}
		\draw [->] (-5, 0) -- (5, 0) node [right] {$x$};
		\draw [->, use as bounding box] (0, -2.5) -- (0, 2.5) node [above] {$f(x)$};
		\draw node at (-4.5,0) [below] {$ -6 \pi$}; 
		\draw node at (-3,0) [below] {$ -4 \pi$}; 
		\draw node at (-1.5,0) [below] {$ -2 \pi$}; 
		\draw node at (1.5,0) [below] {$ 2 \pi$}; 
		\draw node at (3,0) [below] {$ 4 \pi$}; 
		\draw node at (4.5,0) [below] {$ 6 \pi$}; 
		
		\end{tikzpicture}
	\end{center}

\end{enumerate}

Fourier series for $ g(x) = 2x $ (odd function) in the range $ (-\pi,\pi) $ given by


\[ \frac{f(x_{+} + f(x_{-}))}{2} =  \sum_{n=1}^{\infty} b_{n} \sin  n x   \]

where 
\begin{align*}
b_{n} & = \frac{1}{L} \int_{-L}^{L} f(x) \sin \left( \frac{n \pi x}{L} \right) \; \d x  \\
& = \frac{2}{\pi} \int_{-\pi}^{\pi} x \sin n x \; \d x
\end{align*}

Integrating by parts,

\begin{align*}
\int_{-\pi}^{\pi} x \sin n x \; \d x & = \left[  \frac{- x \cos n x}{n} + \frac{1}{n} \int \cos n x \; \d x \right]_{-\pi}^{\pi} \\
& = \frac{- 2 \pi \cos n \pi}{n} + \frac{1}{n} \left[ \frac{\sin n x}{n \pi} \right]_{-\pi}^{\pi} \\
& = \frac{- 2 \pi (-1)^{n}}{n}
\end{align*}

Whence 

\[ g(x) = \sum_{n=1}^{\infty} \frac{ 4 \pi^{2} (-1)^{n+1}}{n^{2}} \sin  n x  \]


Fourier series for $ h(x) = 2| x | $ (even function) in the range $ (-\pi,\pi) $ given by


\[ \frac{f(x_{+} + f(x_{-}))}{2} =  \frac{1}{2} a_{0} +  \sum_{n=1}^{\infty} a_{n} \cos  n x   \]


where 

\begin{align*}
\frac{1}{2} a_{0} & = \frac{1}{2L} \int_{-L}^{L} f(x) \; \d x \\
& = \frac{1}{2\pi} \int_{-\pi}^{\pi} 2| x | \; \d x \\
& = \frac{2}{\pi} \int_{0}^{\pi} x \; \d x \\
& = \pi
\end{align*}
and 
\begin{align*}
a_{n} & = \frac{1}{L} \int_{-L}^{L} f(x) \cos \left( \frac{n \pi x}{L} \right) \; \d x  \\
& = \frac{2}{\pi} \int_{-\pi}^{\pi} | x | \cos n x \; \d x
\end{align*}





Integrating by parts,

\begin{align*}
\int_{-\pi}^{\pi} | x | \cos n x \; \d x & = 2 \int_{0}^{\pi} x  \cos n x \; \d x \\
& = 2 \left[ \frac{x \sin n x}{n} - \frac{1}{n} \int \sin n x \; \d x \right]_{0}^{\pi}  \\
& = - \frac{2}{n} \int_{0}^{\pi} \sin n x \; \d x \\
& = - \frac{2}{n} \left[ - \frac{\cos n x}{n} \right]_{0}^{\pi}\\
& = \frac{2}{n^{2}} (\cos n \pi - 1) 
\end{align*}

Whence

\[ h(x) = \pi +  \sum_{n=1}^{\infty} \frac{2}{n^{2}} ((-1)^{n} - 1)  \cos  n x \]







\section{QUESTION 3}


$ f(x) = e^{x} $ on $ (-\pi,\pi) $ has Fourier series given by 


\[ \frac{f(x_{+} + f(x_{-}))}{2} = \frac{1}{2} a_{0} + \sum_{n=1}^{\infty} \left[ a_{n} \cos n x + b_{n} \sin n x  \right]  \]


where 

\begin{align*}
\frac{1}{2} a_{0} & = \frac{1}{2\pi} \int_{-\pi}^{\pi} e^{x} \; \d x \\
& = \frac{1}{2\pi} \left(  e^{\pi} - e^{-\pi} \right) \\
& = \frac{1}{\pi} \sinh \pi
\end{align*}
and 
\begin{align*}
a_{n} & = \frac{1}{\pi} \underbrace{ \int_{-\pi}^{\pi} e^{x} \cos n x \; \d x}_{I_{a}}  \\
I_{a} & =  \left[   e^{x} \cos n x + \int e^{x} n \sin n x  \; \d x  \right]_{-\pi}^{\pi} \\
& = (e^{\pi} - e^{-\pi}  )\cos n \pi + n \int_{-\pi}^{\pi} e^{x} \sin n x \;\d x \\
& = 2 \sinh \pi \;  (-1)^{n} + n \left[  e^{x} \sin n x - \int e^{x} n \cos x \; \d x  \right]_{-\pi}^{\pi} \\
& =  2 \sinh \pi \;  (-1)^{n} + -n^{2} \int_{-\pi}^{\pi} e^{x} \cos n x \; \d x \\
& =  2 \sinh \pi \;  (-1)^{n} + -n^{2} I_{a}
\end{align*}

Hence 

\[ a_{n} = \frac{2}{\pi} \frac{1}{1 + n^{2}}  \sinh \pi \; (-1)^{n} \]

\section{QUESTION 4}

\begin{enumerate}
	\item Reposing the Fourier Series of $ f(t) $ using complex variables,
	
	\begin{align*}
	f(t) & = \frac{a_{0}}{2} + \sum_{n=1}^{\infty}  \left[   \frac{a_{n}}{2} \left(   e^{\frac{i n \pi t}{L}} + e^{\frac{- i n \pi t}{L}} \right) + \frac{b_{n}}{2i} \left( e^{\frac{i n \pi t}{L}} - e^{\frac{-i n \pi t}{L}} \right)   \right]  \\
	& = \sum_{n=-\infty}^{\infty}  c_{n} e^{\frac{i n \pi t}{L}}, \\
	c_{n} & = \frac{a_{n} - i b_{n}}{2} \; n > 0 ; \\
	c_{-n} & = \frac{a_{n} + i b_{n}}{2} \; n > 0 ; \\
	c_{0} & = \frac{a_{0}}{2}
	\end{align*}
	
	Using the orthogonality of complex exponentials and the properties of complex Fourier coefficients, we deduce that
	
	\begin{align*}
	\int_{-L}^{L} \left[  f(t) \right]^{2} \; \d t  & = \sum_{n = - \infty}^{\infty} \sum_{m = -\infty}^{\infty} c_{n} c_{m} \int_{-T}^{T} \exp \left[   \frac{i \pi t (n + m)}{L} \right]  \; \d t \\
	& = \sum_{n = - \infty}^{\infty} \sum_{m = -\infty}^{\infty} c_{n} c_{m} 2 T \delta_{n[-m]}  \; \\ 
	& = 2 T \sum_{n = - \infty}^{\infty} c_{n} c_{-n} \\
	& = 2 T \sum_{n = - \infty}^{\infty} c_{n} c_{n}^{*} \\
	& = 2 T \sum_{n = - \infty}^{\infty} | c_{n} |^{2} \\
	\end{align*}
	
	This can be then re-expressed in terms of the $ a_{n} $ and $ b_{n} $ as 
	
	\[ \int_{-L}^{L} \left[  f(t) \right]^{2} \; \d t  = L  \left[   \frac{a_{0}^{2}}{2} +\sum_{n=1}^{\infty} (a_{n}^{2} + b_{n}^{2}) \right]  \]
	
	as required. 
	 
	\item 
	
\end{enumerate}



\section{QUESTION 5}

\section{QUESTION 6}

Call $ -\d^{2} / \d x^{2} = \mathcal{L} $, and search for solutions to:

\[ \mathcal{L} y_{n} = \lambda_{n} y_{n}, \quad y_{n}(0) = 0, \;  y_{n}(1) + y_{n}'(1) = 0  \]
      
Then  
      
\[ y_{n}'' + \lambda_{n} y_{n} = 0 \Rightarrow y_{n} = A \cos \sqrt{\lambda} x + B \sin \sqrt{\lambda} x \]

$ y_{n}(0) = 0 \Rightarrow A = 0 $, and the second condition implies

\[ B \sin \sqrt{\lambda_{n}} + B \sqrt{\lambda_{n}} \cos \sqrt{\lambda_{n}} = 0 \]

$ B \neq 0 $, so we have $ \sqrt{\lambda_{n}} = - \tan \sqrt{\lambda_{n}}  $,

so eigenvalues are given by the squares of the solutions to $ \xi = - \tan \xi $, $ \xi > 0 $

\section{QUESTION 7}

\section{QUESTION 8}




\section{QUESTION 9}





\end{document}