	\documentclass[a4paper]{article}
\usepackage{amsmath}
\def\npart {IA}
\def\nterm {Michaelmas}
\def\nyear {2017}
\def\nlecturer {Mx Tsang (jmft2@cam.ac.uk)}
\def\ncourse {Variational Principles Example Sheet 2}

\input{header}

\newtheorem*{soln}{Solution}

\renewcommand{\thesection}{}
\renewcommand{\thesubsection}{\arabic{section}.\arabic{subsection}}
\makeatletter
\def\@seccntformat#1{\csname #1ignore\expandafter\endcsname\csname the#1\endcsname\quad}
\let\sectionignore\@gobbletwo
\let\latex@numberline\numberline
\def\numberline#1{\if\relax#1\relax\else\latex@numberline{#1}\fi}
\makeatother


\begin{document}
	
\maketitle

\section{QUESTION 1}

\begin{align*}
F[x + \delta x] - F[x] & = \int_{t_{1}}^{t_{2}} f(x + \delta x, \dot{x} + \delta \dot{x}, \ddot{x} + \delta \ddot x, t ) \; \d t - \int_{t_{1}}^{t_2} f(t,x,\dot{x},\ddot{x}) \; \d t   \\
& = \int_{t_{1}}^{t_{2}} \left\{  \delta x \frac{\partial f }{\partial x} + (\delta \dot{x}) \frac{\partial f }{\partial \dot{x}} + (\delta \ddot{x}) \frac{\partial f }{\partial \ddot{x}}  \right\} \; \d t + O(t^{2})
\end{align*}

Discarding the (small )terms of $ O(t^{2}) $, we call the first order variation $ \delta F[x] $ and integrating by parts (twice), we have

\begin{align*}
\delta F[x]  & = \int_{t_{1}}^{t_{2}} \left\{   \delta x \left[   \frac{\partial f }{\partial x }  - \frac{\d }{\d t} \left(  \frac{\partial f }{\partial \dot{x}} \right)    \right]  - (\delta \dot{x}) \frac{\d }{\d t} \left(  \frac{\partial f }{\partial \ddot{x}} \right)   \right\} \; \d t + \left[  \delta x \frac{\partial f }{\partial \dot{x}} + ( \delta \dot{x}) \frac{\partial f }{\partial \ddot{x}} \right]_{t_{1}}^{t_{2}}   \\
& = \int_{t_{1}}^{t_{2}} \left\{   \delta x \left[   \frac{\partial f }{\partial x }  - \frac{\d }{\d t} \left(  \frac{\partial f }{\partial \dot{x}} \right)  +  \frac{\d^{2} }{\d t^{2}} \left(  \frac{\partial f }{\partial \ddot{x}} \right)   \right] \right\} \; \d t\\
& \quad + \left[  \delta x \left\{  \frac{\partial f }{\partial \dot{x}} - \frac{\d }{\d t} \left(  \frac{\partial f }{\partial \ddot{x}} \right)  \right\}  + ( \delta \dot{x}) \frac{\partial f }{\partial \ddot{x}}  \right]_{t_{1}}^{t_{2}}
\end{align*}

We have fixed end boundary conditions, so $ \delta x(t_{1}) = \delta x(t_{2}) = 0 $ and also $ \delta \dot{x} (t_{1}) = \delta \dot{x} (t_{2}) = 0  $. Thus the boundary term is zero and we can write $ \delta F[x] $ in the form


\[ \delta F[x] = \int_{t_{1}}^{t_{2}} \left\{ \delta x(t) \frac{ \delta F[x]}{\delta x(t)}  \right\}  \; \d t  \]


where the \emph{functional derivative} $ \frac{ \delta F[x]}{\delta x(t)} $ is defined as 


\[ \frac{ \delta F[x]}{\delta x(t)} := \frac{\partial f }{\partial x} -  \frac{\d }{\d t} \left(  \frac{\partial f }{\partial \dot{x}} \right)  +  \frac{\d^{2} }{\d t^{2}} \left(  \frac{\partial f }{\partial \ddot{x}} \right)   \]

The functional $ F $ is stationary when its functional derivative is zero ( assuming that this derivative is defined on $ (t_{1},t_{2}) $) and the condition for this to be true is the following Euler-Lagrange equation:

\[ \frac{\partial f }{\partial x} -  \frac{\d }{\d t} \left(  \frac{\partial f }{\partial \dot{x}} \right)  +  \frac{\d^{2} }{\d t^{2}} \left(  \frac{\partial f }{\partial \ddot{x}} \right) = 0, \qquad t_{1} < t < t_{2} \]


Given the functional

\[ L[x] = \int_{1}^{2} t^{4}  [\ddot{x}(t)]^{2} \; \d t  \]

In this case, $ f =  t^{4} [\ddot{x}(t)]^{2}  $, so $   \frac{\partial f }{\partial x} = \frac{\partial f }{\partial \dot{x}} = 0 $ and the EL equation can be immediately twice integrated to give 

\[ \frac{\partial }{\partial \ddot{x}} \left[ t^{4} [\ddot{x}(t)]^{2} \right] = At + B   \]

for some constants $ A $ and $ B $.

ie.

\[  2 t^{4}  \ddot{(x)}(t) = At + B \]
\[ \Rightarrow \ddot{x}(t) = At^{-3} + B t^{-4} \qquad t \neq 0 \]

\[ \Rightarrow \dot{x}(t) = A' t^{-2} + B' t^{-3} + C \]
Using b.c.s we have

\[ -2 = A' + B' + C \]
\[ -\frac{1}{4} = \frac{1}{4} A' + \frac{1}{8} B' + C \Rightarrow -2 = 2 A' + B' + 8C \]

Subtracting immediately yields $ A' = 7 C $:

\[ -2 = 8 C + B' \]
\[ -2 = 22C + B' \]

Therefore $ C' = 0 $, $ B' = -2 $, and $ \dot{x}(n) = -2 t^{-3} $.

Integrating, we get

\[ x(t) = t^{-2} + D \]

b.c.s $ \Rightarrow D = 0 $, so $ x(t) = \frac{1}{t^{2}} $. 

This function is a global minimum as it is convex. 

Note: $ \delta^{2} F > 0 \not \implies  $ global min. Need to use convexity. of $ \int_{1}^{2} t^{4} [ \ddot{x}(t) ]^{2} \; \d t $. (Clearly convex as we're just doing linear things, then squaring.)

\section{QUESTION 2}


Our aim is to maximise $ A[x,y] $ subject to the constraint $ P[x,y] = L $, where $ L $ is the fixed length and $ P[x,y] = \int_{0}^{2\pi} \sqrt{  (x')^{2}  + (y')^{2} } \; \d \theta  $

Using a Lagrange multiplier $ \lambda $ to impose this, we seek to maximize the functional

\begin{align*}
\phi_{\lambda}[x,y]  & = A[x,y] - \lambda ( P[y] - L )  \\
& = \int_{0}^{2 \pi} \underbrace{\frac{1}{2} ( xy' - yx' ) - \lambda \sqrt{  (x')^{2}  + (y')^{2} }}_{=f_{\lambda}(\mathbf{x},\mathbf{x}')} \; \d \theta + \lambda L
\end{align*}

where $ \mathbf{x} = (x,y) $. The boundary conditions imply that $ x(0) = x(2\pi), x'(0) = x'(2\pi) $ and similarly for y at the endpoints, so boundary terms vanish and functional is stationary for solutions of the E-L equation.  $ f_{\lambda}(\mathbf{x},\mathbf{x}') $ has no explicit $ \theta $ dependence, so considering the $ y $ E-L equation we have that:

\[ f - x'\frac{\partial f_{\lambda} }{\partial x'}  - y'\frac{\partial f_{\lambda} }{\partial y'}  = \text{ constant}  \]

\begin{align*}
& \Rightarrow f - y' \left(  \frac{1}{2} x - \frac{\lambda y'}{\sqrt{  (x')^{2}  + (y')^{2} }} \right)  - x'\left(  - \frac{1}{2} y - \frac{\lambda x'}{\sqrt{  (x')^{2}  + (y')^{2} }}   \right)    = \text{constant} \\
& \Rightarrow  - \lambda \frac{ ( (x')^{2}  + (y')^{2} )}{\sqrt{  (x')^{2}  + (y')^{2} }} + \lambda \frac{(y')^{2}}{\sqrt{  (x')^{2}  + (y')^{2} }} + \lambda \frac{(x')^{2}}{\sqrt{  (x')^{2}  + (y')^{2} }} = \text{constant} \\
& \Rightarrow 0 = C
\end{align*}

Hmm?
Try E-L directly...




\section{QUESTION 3}

Using Lagrange multiplier $ \lambda $, wish to minimize


\begin{align*}
\Phi_{\lambda}[\psi] & = I[\psi] - \lambda  \left[    \int_{-\infty}^{\infty}  \psi^{2} \; \d x = 1  \right] \\
& = \int_{-\infty}^{\infty} \underbrace{(\psi')^{2} + (x^{2} - \lambda  ) \psi^{2} }_{f_{\lambda}(\psi,\psi' ; x)} \; \d x + \lambda
\end{align*}

Normalisation condition, can assume $ \phi = 0 $ at endpoints, so the functional is stationary for solutions of the E-L equation.
Euler-Lagrange equations imply:

\[ 2(x^{2} - \lambda) \psi - \frac{\d }{\d x} \left[  2 \psi' \right] = 0  \]

\[ \Rightarrow \psi'' + (x^{2} - \lambda) \psi = 0 \]

Note that

\begin{align*}
I[\psi]  & =  \int_{-\infty}^{\infty}  (\psi' + x^{2} \psi^{2} )^{2} - 2 x \psi \psi' \; \d x    \\
& =  \int_{-\infty}^{\infty}  (\psi' + x^{2} \psi^{2} )^{2} \; \d x  - \int_{-\infty}^{\infty}  x \frac{\d }{\d x}[\psi^{2}] \; \d x \\
& =  \int_{-\infty}^{\infty}  (\psi' + x^{2} \psi^{2} )^{2} \; \d x  - \left[     x \psi^{2} \right]_{-\infty}^{\infty} + \int_{-\infty}^{\infty} \psi^{2} \; \d x  \quad \text{by parts} \\
& =   \int_{-\infty}^{\infty}  (\psi' + x^{2} \psi^{2} )^{2} \; \d x + 1   \end{align*}

As $ (\psi' + x^{2} \psi^{2}) $ is real valued, its square gives a positive function, thus the integral is positive and $ I[\psi] \geq 1 $. Equality holds for 

\begin{align*}
& \quad \; \; (\psi' + x \psi) = 0 \\
& \Rightarrow \psi'+ x \psi = 0 \\
& \Rightarrow \frac{\d }{\d x}  \left( \psi e^{x^{2}/2} \right) = 0 \\
& \Rightarrow \psi = C e^{- x^{2} / 2 }  
\end{align*}

for some constant $ C $ (which we recognise as the Gaussian Wave Function).
The normalisation condition implies that $ C = \left(  \frac{1}{\pi} \right)^{1/4}  $. 

Note: We're minimising the energy of a harmonic oscillator. What does $ \lambda $ represent here?





\section{QUESTION 4}
                                                 
Using Lagrange multiplier $ \lambda $ with constraint $ | \mathbf{x} | = 1 $. We will instead use the equivalent constraint $ | \mathbf{x} |^{2} = 1 $, so we wish to minimize the functional 
                                                 
\begin{align*}
\Phi_{\lambda}[\mathbf{x}] & = I[\mathbf{x}] - \lambda(t) (  | \mathbf{x} |^{2} - 1 ) \\
& = \int_{t_{1}}^{t_{2}} \underbrace{| \dot{\mathbf{x}} |^{2} - \lambda(t) | \mathbf{x} |^{2}}_{f_{\lambda}(\mathbf{x},\dot{\mathbf{x}} ; t )  } \; \d t + \lambda
\end{align*}   

The E-L equation for $ x_{i} $ component is $ \frac{\partial f }{\partial x_{i}} - \frac{\d }{\d t} \left(  \frac{\partial f}{\partial \dot{x}_{i}} \right) = 0   $. Have


\begin{align*}
\frac{\partial f }{\partial x_{i}} & = - \lambda(t) \frac{\partial }{\partial x_{i}} (x_{j}x_{j})  \\
& = - 2 \lambda(t) x_{j} \underbrace{\frac{\partial x_{j}}{\partial x_{i}}}_{\delta_{ij}} \\
& = - 2 \lambda(t) x_{i} \\
\frac{\d }{\d t} \left(  \frac{\partial f}{\partial \dot{x}_{i}} \right) & = \frac{\d }{\d t} \left( 2 \dot{x}_{i}  \right) \\
& = 2 \ddot{x}_{i}  
\end{align*}

So E-L gives

\begin{align*}
\ddot{x_{i}} + \lambda(t) x_{i} & = 0 \\
\Rightarrow  \ddot{\mathbf{x}} + \lambda(t) \mathbf{x} & = \mathbf{0}  \qquad (*)
\end{align*}    

Take the constraint $ | \mathbf{x} |^{2} = 1 $ and differentiate to get

\[ 2 \dot{\mathbf{x}} \cdot \mathbf{x} = \mathbf{0} \]

Cancelling the two and differentiating again gives

\[ \ddot{\mathbf{x}}  \cdot \mathbf{x} + | \mathbf{\dot{x}} |^{2} = \mathbf{0} \]

Dotting (*) with $ \mathbf{x} $ gives

\[  \ddot{\mathbf{x}}  \cdot \mathbf{x} + \lambda(t) \underbrace{ | \mathbf{x} |^{2}}_{=1} = \mathbf{0} \]

Hence comparing gives $ \lambda(t) =  | \mathbf{\dot{x}} |^{2} $ and thus the desired equation

\[ \ddot{\mathbf{x}} +  | \mathbf{\dot{x}} |^{2} \mathbf{x}  = \mathbf{0}\]
   

 
 
                




\section{QUESTION 5}


Have the Lagrangian

\[ L = \underbrace{\frac{1}{2} m a^{2} \dot{\theta}^{2}  + \frac{1}{2} m a^{2} \dot{\theta}^{2}  }_{T} + \underbrace{mga \cos \theta}_{- V} \]

Note that $ \frac{\partial L}{\partial \phi} = 0 $ so we have the first integral

\[ \text{const. } = \frac{\partial L }{\partial \dot{\phi}} = m a^{2} \sin^{2} \theta  \]

Note too that $ \frac{\partial L }{\partial t} = 0 $ (no t dependence) so we have another first integral

\begin{align*}
\text{const. } & = L - \dot{\phi} \frac{\partial L }{\partial \dot{\phi}} - \dot{\theta} \frac{\partial L }{\partial \dot{\theta}} \\
& = - T - V
\end{align*}

from which we deduce that

\[ \frac{1}{2} m a^{2} \dot{\theta}^{2}  + \frac{1}{2} m a^{2} \dot{\theta}^{2}  - mga \cos \theta = E \]

for the total energy.

The Hamiltonian is defined as the Legendre transform of the Lagrangian with respect to velocity $ \mathbf{v} = \dot{\mathbf{x}} $:

\[ H(\mathbf{x},\mathbf{p};t)  = [ \mathbf{p} \cdot \mathbf{v}  - L(\mathbf{x},\mathbf{v}) ]_{\mathbf{v} = \mathbf{v(\mathbf{p})}} \]

where $ \mathbf{v}(\mathbf{p}) $ is the solution to $ \frac{\partial L }{\partial \mathbf{v}} = \mathbf{p} $.

The momentum $ p_{\theta} $ is given by

\begin{align*}
p_{\theta}  & = \frac{\partial  L}{\partial \dot{\theta}} \\
& = m a^{2} \dot{\theta}
\end{align*}

Similarly,

\begin{align*}
p_{\phi} & = \frac{\partial  L}{\partial \dot{\phi}}  \\
& = m a^{2} (\sin^{2} \theta ) \dot{\phi}
\end{align*}

Thus $ \mathbf{v} = (\dot{\theta},\dot{\phi}) = \left(  \frac{p_{\theta}}{ma^{2}},  \frac{p_{\phi}}{ma^{2}\sin^{2}\theta   } \right)   $ and

\begin{align*}
H & = \frac{p_{\theta}^{2}}{ma^{2}} +  \frac{p_{\phi}^{2}}{ma^{2}\sin^{2}\theta } - \left(  \frac{1}{2} m a^{2} \left(  \frac{p_{\theta}}{ma^{2}}\right)^{2}   + \frac{1}{2} m a^{2} \left( \frac{p_{\phi}}{ma^{2}\sin^{2}\theta } \right)^{2}  + mga \cos \theta  \right)    \\
& =  \frac{1}{2} \frac{p_{\theta}^{2}}{ma^{2}} + \frac{1}{2} \frac{p_{\phi}^{2}}{ma^{2}\sin^{2}\theta } -mga \cos \theta
\end{align*}

Hamilton's equations are given by

\[ \dot{\mathbf{x}} = \frac{\partial H }{\partial \mathbf{p}}, \qquad \dot{\mathbf{p}} = - \frac{\partial H }{\partial \mathbf{x}}   \]

ie.

\[ \dot{\theta}  = \frac{p_{\theta}}{ma^{2}} \]
\[ \dot{\phi}  = \frac{p_{\phi}}{ma^{2} \sin^{2} \theta } \]

\[ \dot{p_{\theta}} = \frac{-p_{\phi}^{2} \sin(2\theta) }{2 ma^{2} \sin^{4} \theta}  - mga \cos \theta \]
\[ \dot{p_{\phi}} = 0 \]

\section{QUESTION 6}

\begin{enumerate}
	\item Consider the variation directly, $ u_{t} \to u_{t} + (\delta u)_{t} $ and $ u_{x} \to u_{x} + (\delta u)_{x} $. Then
	
	\begin{align*}
	\delta I[u] & = I[u + \delta u] - I[u] \\
	& = \int \left[ \frac{1}{2}\left(  u_{t} + (\delta u)_{t} \right)^{2} - F(u_{x} + (\delta u)_{x}) \right]  \; \d x \; \d t - \int \left[  \frac{1}{2} u_{t}^{2} - F(u_{x}) \; \d x \; \d t    \right]\\
	& = \int u_{t} (\delta u)_{t} - (\delta u)_{x} \frac{\partial F(u_{x}) }{\partial u_{x}} \; \d x \; \d t +   O(t^{2}) \\
	& = \int u_{tt} (\delta u) - (\delta u) \frac{\d }{\d x} \left[ \frac{\partial F(u_{x})  }{\partial u_{x}} \right]  \; \d x \; \d t + \text{boundary terms} \qquad \text{(by parts)}
	\end{align*}
	
	ignoring boundary terms
	
	So the Euler-Lagrange equation is 
	
	\[ \frac{\partial^{2} u}{\partial t^{2}} - \frac{\d }{\d x} \left[  \frac{\partial F(u_{x}) }{\partial u_{x}} \right]   = 0  \]
	
	ie $ u_{tt} = u_{xx} \frac{\partial^{2} F }{\partial u_{x}^{2}} $
	
	\item 
	
	Discarding second order terms throughout:
	
	\begin{align*}
	\delta I[u] & = \int \left[ (u_{x} + (\delta u)_{x})^{2} + (  u_{y} + (\delta u)_{y} )^{2} + e^{2(u + \delta u)}  \right] \; \d x \; \d y - \int u_{x}^{2} + u_{y}^{2} + e^{2u} \; \d x \; \d y   \\
	& = \int 2 u_{x} (\delta u)_{x} + 2 u_{y} ( \delta u)_{y} + \left(  e^{2(u + \delta u)} - e^{2u} \right) \; \d x \; \d y + O(u^{2}) \\
	& = \int 2 u_{x} (\delta u)_{x} + 2 u_{y} ( \delta u)_{y} + e^{2u}\left( 1 + 2 \delta u \right) - e^{2u}  \; \d x \; \d y  \qquad \text{ using } e^{x} \approx 1 + x\\
	& = 2 \int (\delta u) \{ u_{xx} + u_{yy}  + 2 e^{2u} \} \; \d x \; \d y
	\end{align*}
	
	So E-L equation is 
	
	\[ \nabla^{2} u  = -2e^{u}  \]
	
	
	
	
	
\end{enumerate}


\section{QUESTION 7}

The E-L equations are of the form $ \frac{\partial L }{\partial x_{i} } - \frac{\d }{\d t} \left(  \frac{\partial L}{\partial \dot{x}_{i}} \right) = 0 $

We have
\[ \frac{\partial L }{\partial x_{i}} = - q \nabla_{i} \phi + q \frac{\partial }{\partial x_{i}} (\mathbf{v} \cdot \mathbf{A}) \]

and

\[ \frac{\partial L }{\partial \dot{x}_{i}} = m \gamma v_{i} + q A_{i} \]


E-L equations imply

\begin{align*}
& \quad \quad - q \nabla_{i} \phi + q \frac{\partial }{\partial x_{i}} (\mathbf{v} \cdot \mathbf{A}) - \frac{\d }{\d t}  \left(  m \gamma v_{i} + q A_{i} \right) = 0   \\
& \Rightarrow  \frac{\d }{\d t}  \left(  m \gamma v_{i} \right) = - q \nabla_{i} \phi + q \frac{\partial }{\partial x_{i}} (\mathbf{v} \cdot \mathbf{A}) - q \frac{\d }{\d t}( A_{i})
 \end{align*}
 
 
Using the chain rule:
 
\begin{align*}
\frac{\d A_{i}}{\d t} & = \frac{\partial A_{i} }{\partial t} \frac{\d t}{\d t } + \frac{\partial A_{i} }{\partial x_{j}} \frac{\d x_{j}}{\d t} \\
& = \frac{\partial A_{i} }{\partial t} +  v_{j} \frac{\partial A_{i} }{\partial x_{j}} 
\end{align*}

and

\[ \frac{\partial }{\partial x} (\mathbf{v} \cdot \mathbf{A}) = v_{j} \frac{\partial A_{j} }{\partial x_{i}}  \]


\begin{align*}
\Rightarrow  \frac{\d }{\d t}  \left(  m \gamma v_{i} \right) & = - q \nabla_{i} \phi + q v_{j} \frac{\partial A_{j} }{\partial x_{i}} - q \left[  \frac{\partial A_{i} }{\partial t} +  v_{j} \frac{\partial A_{i} }{\partial x_{j}} \right] \\
 & = q \left( \underbrace{\nabla_{i} \phi - \frac{\partial A_{i} }{\partial t}}_{E_{i}}  + \underbrace{\left[ v_{j} \frac{\partial A_{j} }{\partial x_{i}}  -  v_{j} \frac{\partial A_{i} }{\partial x_{j}} \right]}_{(*)}    \right)  
\end{align*}

Lastly, want to show (*) is equal to $[  \mathbf{v} \times \mathbf{B}  ]_{i} = [\mathbf{v} \times \nabla \times A ]_{i}   $

\begin{align*}
[\mathbf{v} \times \nabla \times A ]_{i} & = \varepsilon_{ijk} v_{j} [nabla \times A ]_{k}  \\
& = \varepsilon_{kij}\varepsilon_{kpq} v_{j} \frac{\partial A_{q} }{\partial x_{p}}  \\
& = \delta_{ip}\delta_{jq} v_{j} \frac{\partial A_{q} }{\partial x_{p}} - \delta_{iq}\delta_{jp} v_{j} \frac{\partial A_{q} }{\partial x_{p}} \\
& = \frac{\partial A_{i} }{\partial t} +  v_{j} \frac{\partial A_{i} }{\partial x_{j}}
\end{align*}

as required.


\section{QUESTION 8}


\[ S[\rho, \mathbf{v},\phi] =  \int  \d t \;  \int \d^{3}  x  \;  \left\{  \frac{1}{2} \rho | \mathbf{v} |^{2} - u(\rho) + \phi [   \dot{\rho} + \nabla \cdot ( \rho \mathbf{v}) ] \right\}  \]

Note we need a Lagrange multiplier field $ \phi(t,\mathbf{x}) $ to impose the condition at an infinite number of points. This looks like an action for sure (KE + PE). We will have 2 E-L equations, one from varying $ \rho $ and the other from varying $ \mathbf{v}  $.



Taking variations directly,

\begin{align*}
S[\rho + \delta \rho , \mathbf{v},\phi] & = S[\rho, \mathbf{v},\phi] + \int  \d t \;  \int \d^{3}  x  \;  \left\{  \frac{1}{2} \delta \rho | \mathbf{v} |^{2} - \delta \rho \frac{\partial u }{\partial \rho} + \phi [   \dot{\delta \rho} +  \nabla \cdot ( \delta \rho \mathbf{v}) ] \right\} \\
& = \end{align*}
\section{QUESTION 9}


\section{QUESTION 10}
\section{QUESTION 11}









\end{document}