\documentclass[a4paper]{article}
\usepackage{amsmath}
\def\npart {IB}
\def\nterm {Michaelmas}
\def\nyear {2017}
\def\nlecturer {Dr Warnick}
\def\ncourse {Quantum Mechanics Example Sheet 2}

\input{header}
\newtheorem*{soln}{Solution}

\renewcommand{\thesection}{}
\renewcommand{\thesubsection}{\arabic{section}.\arabic{subsection}}
\makeatletter
\def\@seccntformat#1{\csname #1ignore\expandafter\endcsname\csname the#1\endcsname\quad}
\let\sectionignore\@gobbletwo
\let\latex@numberline\numberline
\def\numberline#1{\if\relax#1\relax\else\latex@numberline{#1}\fi}
\makeatother


\begin{document}
	
\maketitle

\section{QUESTION 1}


The potential $ V(x) = 0 $ so our time independent SE is:

\[ -\frac{\hbar^{2}}{2m} \frac{\d^{2} \psi}{\d x^{2}} = E \psi  \]

\[ \iff \psi'' + k^{2} \psi = 0 \]

setting $ E = k^{2} \hbar^{2} / 2m $, thus 

\[ \psi(x) = A \cos k x + B \sin k x \]

Using BCs, $ \psi(0) = 0 \Rightarrow A = 0 $

$ \psi(a) = 0 \Rightarrow \sin k a = 0 \Rightarrow k a =  n \pi  $ for integer $ n $, thus energy eigenvalues are $ E_{n} = n^{2} \pi^{2} \hbar^{2} / 2m a^{2} $ with corresponding energy eigenstates $ B_{n} \sin k_{n} x = B_{n} \sin ( \sqrt{2 m a^{2 }E_{n} / \hbar^{2} } x ) $, and 

\begin{align*}
1 & = \int_{0}^{a} |  \psi(x) |^{2} \; \d x \\
& = \int_{0}^{a} B_{n}^{2} \sin^{2} ( k_{n} x ) \; \d x  \\
& = B_{n}^{2} \left[  \frac{x}{2}  - \frac{1}{4} \sin ( 2 k_{n} x ) \right]_{0}^{a} \\
& = B_{n}^{2} \frac{a}{2}
\end{align*}

\begin{align*}
\Rightarrow \; & B_{n}  = \sqrt{\frac{2}{a}} \\
\Rightarrow & \text{ norm. states are } \psi_{n}(x) = \sqrt{\frac{2}{a}} \sin \left(    \sqrt{\frac{2m a^{2} E_{n}}{\hbar^{2}} } x \right)
\end{align*} 

Let $ \psi_{n} $ denote the expectation value of $ \hat{x} $ in state $ \psi_{n} $, then

\begin{align*}
\langle \hat{x} \rangle_{n} & = (\psi_{n},\hat{x} \psi_{n} )  \\
& = \int_{0}^{a} \psi_{n}^{*} x \psi_{n} \; \d x \\
& = \frac{2}{a} \int_{0}^{a}  x \sin^{2} k_{n} x \; \d x \\
\end{align*}

By parts,

\begin{align*}
\int_{0}^{a}  x \sin^{2} k_{n} x \; \d x & = \left[  \frac{x^{2}}{2}  - \frac{1}{4 k_{n}} x \sin ( 2 k_{n} x ) \right]_{0}^{a} - \int_{0}^{a} \frac{x}{2}  - \frac{1}{4 k_{n}} \sin ( 2 k_{n} x ) \; \d x \\
& = \frac{a^{2}}{2} - \left[  \frac{x^{2}}{4}  + \frac{1}{8 k_{n}^{2}} \cos(2 k_{n} x)  \right]_{0}^{a} \\
& = \frac{a^{2}}{2} - \left[  \frac{x^{2}}{4}  + \frac{1}{8 k_{n}^{2}} \left( 1 - \sin^{2} (k_{n} x )   \right) \right]_{0}^{a}\\
& = \frac{a^{2}}{2} -  \frac{a^{2}}{4} \\
& = \frac{a^{2}}{4}
\end{align*}
  
Thus $ \langle \hat{x} \rangle_{n} = a / 2 $ as required.

Next, uncertainty of measurement of $ \hat{x} $ in state $ \psi $ given by

\begin{align*}
(\Delta x)_{n}^{2} & = \langle \hat{x}^{2} \rangle_{\psi} -  \langle \hat{x} \rangle_{\psi}^{2} \\
& = \frac{2}{a} \int_{0}^{a} x^{2} \sin^{2} (k_{n} x ) \; \d x - \frac{a^{2}}{4}
\end{align*}

By parts,

\begin{align*}
\int_{0}^{a} x^{2} \sin^{2} (k_{n} x ) \; \d x & = \left[  \frac{x^{3}}{2} - \frac{1}{4 k_{n}} x^{2} \sin(2k_{n} x)     \right]_{0}^{a} - \int_{0}^{a} x^{2} - \frac{1}{2 k_{n} } x \sin(2 k_{n} x) \; \d x    \\
& = \frac{a^{3}}{2} - \frac{a^{3}}{3} + \frac{1}{2 k_{n}} \int_{0}^{a} x \sin(2 k_{n} x) \;  \d x \\
& = \frac{a^{3}}{6} + \frac{1}{2 k_{n}} \left(  \left[  - \frac{1}{2 k_{n}} x \cos(2k _{n} x)  \right]_{0}^{a} + \frac{1}{2k_{n}} \int_{0}^{a} \frac{1}{2k_{n}} \cos(2k_{n} x) \; \d x  \right) \\
& = \frac{a^{3}}{6} - \frac{a}{4k_{n}^{2}} \cos (2 k_{n} a) \\
& = \frac{a^{3}}{6} - \frac{a}{4k_{n}^{2}} \left(  1 - \sin^{2} k_{n} a \right) \\
& =  \frac{a^{3}}{6}  - \frac{a^{3}}{4 n^{2}\pi^{2}}
\end{align*}

Hence

\begin{align*}
(\Delta x)_{n}^{2} & = \frac{a^{2}}{3}  - \frac{a^{2}}{2 n^{2}\pi^{2}}  - \frac{a^{2}}{4} \\
& = \frac{a^{2}}{12} \left( 1 - \frac{6}{\pi^{2} n^{2}} \right) 
\end{align*}

as required.



\section{QUESTION 2}


Harmonic oscillator, mass $ m $, frequency $ \omega $, has potential $ V(x) = \frac{1}{2} m \omega^{2} x^{2} $, hence Hamiltonian is given by

\[ H \psi = - \frac{\hbar^{2}}{2m} \psi'' + \frac{1}{2} m \omega^{2} x^{2} \psi  \]

Writing $ H $ in terms of momentum and position operators, we show that

\begin{align*}
\langle H \rangle_{\psi} & = ( \psi, H \psi )  \\
& = ( \psi,  \frac{1}{2m} \hat{p}^{2} \psi + \frac{1}{2} m \omega^{2} \hat{x}^{2} \psi   ) \\
& = \frac{1}{2m} ( \psi, \hat{p}^{2} \psi) + \frac{1}{2} m \omega^{2} (\psi, \hat{x}^{2} \psi) \\
& = \frac{1}{2m} \left(  (\Delta p)_{\psi}^{2} + \langle \hat{p} \rangle_{\psi}^{2}  \right)  + \frac{1}{2} m \omega^{2} \left(  ( \Delta x)_{\psi}^{2} + \langle \hat{x} \rangle_{\psi}^{2}  \right)
\end{align*}

Energy eigenvalues given by


\begin{align*}
\langle H \rangle_{\psi} & \geq \frac{1}{2m} (\Delta p)_{\psi}^{2} +   + \frac{1}{2} m \omega^{2}( \Delta x)_{\psi}^{2} \\
& = \frac{1}{2m} \left( (\Delta p)_{\psi}^{2} +   + m^{2} \omega^{2}( \Delta x)_{\psi}^{2}  \right)  \\
& \geq  \frac{1}{2m} \left(  \hbar m \omega \right) = \frac{\hbar \omega}{2} 
\end{align*}

where the last inequality follows from the uncertainty relation.
\section{QUESTION 3}

Let $  \Psi(x,t) $ be a solution of the time-dependent SE for a free particle ie. $ \Psi(x,t) $ satisfies

\[ i \hbar \dot{\Psi} = - \frac{\hbar^{2}}{2m} \Psi'' \]

Define $ \Phi(x,t) = \Psi(x-ut,t)e^{ikx}e^{-i \omega t} $, and setting $ \Psi(\xi,\eta) = \Psi(x-ut,t) $,

\begin{align*}
\frac{\partial }{\partial t} \Psi(\xi,\eta) & = \frac{\partial \xi }{\partial t} \frac{\partial \Psi }{\partial \xi} + \frac{\partial \eta }{\partial  t}\frac{\partial \Psi}{\partial \eta}  \\
& = - u \frac{\partial \Psi }{\partial \xi} +\frac{\partial \Psi}{\partial \eta} 
\end{align*}

and 

\begin{align*}
\frac{\partial }{\partial x} \Psi(\xi,\eta) & = \frac{\partial \xi }{\partial x} \frac{\partial \Psi }{\partial \xi} + \frac{\partial \eta }{\partial  x}\frac{\partial \Psi}{\partial \eta}  \\
& = \frac{\partial \Psi }{\partial \xi} 
\end{align*}

similarly the second derivative is

\[ \frac{\partial^{2} \Psi }{\partial x^{2}} = \frac{\partial^{2} \Psi }{\partial \xi^{2}}  \]


First calculate time derivatives,

\begin{align*}
\dot{\Phi} &  = e^{ikx} \left(  e^{-i \omega t} \frac{\partial }{\partial t} \Psi(\xi,\eta) - i \omega e^{-i \omega t} \Psi(\xi,\eta)  \right)   \\
& = e^{ikx}e^{-i \omega t} \left(  - u \frac{\partial \Psi }{\partial \xi} +\frac{\partial \Psi}{\partial \eta}   - i \omega \Psi \right) 
\end{align*}

Next, spatial 

\begin{align*}
\Phi'& = e^{- i \omega t} \left(  e^{i k x } \frac{\partial }{\partial x} \Psi(x - ut,t) + i k e^{i k x} \Psi(x-ut,t)  \right)   \\ 
\end{align*}

\begin{align*}
\Phi'' & = e^{- i \omega t} \left(  e^{i k x } \frac{\partial^{2} }{\partial x^{2}} \Psi(x - ut,t) + 2 i k e^{i k x} \frac{\partial }{\partial x}\Psi(x-ut,t)  - k^{2} e^{i k x} \Psi(x-ut,t)  \right)   \\ 
& = e^{- i \omega t}  e^{i k x } \left( \frac{\partial^{2} \Psi }{\partial \xi^{2}} + 2 i k \frac{\partial \Psi }{\partial \xi}  - k^{2} \Psi  \right)   \\ 
\end{align*}


So time-dependent SE becomes

\begin{align*}
i \hbar \left(  - u \frac{\partial \Psi }{\partial \xi} +\frac{\partial \Psi}{\partial \eta}   - i \omega \Psi \right)  & = - \frac{\hbar^{2}}{2m} \left( \frac{\partial^{2} \Psi }{\partial \xi^{2}} + 2 i k \frac{\partial \Psi }{\partial \xi}  - k^{2} \Psi  \right) 
\end{align*}

Linear independence allows us to compare the coefficients of $ \frac{\partial \Psi }{\partial \xi}  $ and $ \Psi $ to obtain

\[ - i \hbar u = - \frac{\hbar^{2}}{2m} 2 i k  \qquad \qquad  \hbar \omega =  \frac{\hbar^{2} k^{2}}{2m} \]

\[  m u = \hbar k \qquad \qquad 2m \omega = \hbar k^{2} \]

Thus $ \Phi $ is a solution if $ k = \frac{m u}{\hbar} $ and $ \omega = \frac{\hbar}{2m} k^{2} = \frac{m u^{2}}{2 \hbar} $

Next, comparing expectation values. 

Note

\begin{align*}
\langle \hat{x} \rangle_{\Psi} & =  (\Psi, \hat{x} \Psi)\\
& = \int_{-\infty}^{\infty} x | \Psi |^{2} \; \d x
\end{align*}

Clearly

\[ | \Phi |^{2} = | \Psi |^{2}  \]

and so

\[ \langle \hat{x} \rangle_{\Phi} = \langle \hat{x} \rangle_{\Psi} \]

But

\begin{align*}
\langle \hat{p} \rangle_{\Phi}& = \int_{-\infty}^{\infty} \Phi^{*} ( - i \hbar \Phi') \; \d x   \\
& = \int_{-\infty}^{\infty} \Psi^{*} ( - i \hbar \Psi') \; \d x  + \int_{-\infty}^{\infty} \Psi^{*} \Psi \; \d x  \\
& = \langle \hat{p} \rangle_{\Psi} + \hbar k
\end{align*}

To show consistency with Ehrenfest's Thm, want to check

\[ \frac{\d }{\d t} \langle \hat{x} \rangle_{\Phi}  = \frac{1}{m} \langle \hat{p}  \rangle_{\Psi}  \]

However since $ \langle \hat{x} \rangle_{\Phi} = \langle \hat{x} \rangle_{\Psi} $, their derivatives must also be equal; this cannot happen as $ \langle \hat{p} \rangle_{\Phi} \neq \langle \hat{p} \rangle_{\Psi} $, so the first part of Ehrenfest's does not hold. 

The next part 

\[ \frac{\d }{\d t} \langle \hat{p} \rangle_{\Phi}  = - \langle V'(\hat{x})  \rangle_{\Psi}  \]

does hold, as the difference in momenta does not depend on $ t $.

\section{QUESTION 4}

We have

\[ H \psi_{n}(x) = E_{n} \psi_{n}(x)  \]

For energy levels $ E_{n} = (n + \frac{1}{2}) \hbar \omega $ with corresponding energy eigenstates $ \psi_{n}(x) = h_{n}(y) e^{-y^{2}/2} $ where $ y = (m \omega / \hbar )^{1/2} x $ and $ h_{n} $ is a polynomial of degree $ n $ with $ h_{n}(-y) = (-1)^{n} h_{n}(y) $, for $ n = 0,1,2,\cdots $

First, $ \psi_{0}(x) = a_{0} e^{- y^{2} / 2} $ for some constant $ a_{0} $.

Know that $ \psi_{2}(x) = a_{2}(y) e^{-y^{2}/2}  $, $ h_{2}(-y) = h_{2}(y) $ even function so $ h_{2}(y) $ is of the from $ Ay^{2} + B $. By orthogonality,

\begin{align*}
0 & = (\psi_{0},\psi_{2}) \\
& = \int_{- \infty}^{\infty} \psi_{0}^{*} \psi_{2} \; \d y  \\
& = \int_{- \infty}^{\infty} a_{0} \left( Ay^{2} + B \right)e^{- y^{2} / 2}    \; \d y \\
& = a_{0} \left( A \sqrt{2 \pi} + B \sqrt{2 \pi}  \right) 
\end{align*}

Thus $ A = - B $, and $ \psi_{2}(x) = a_2(y^{2} - 1) $ for some constant $ a_{2} $. Similarly, can write $ h_{3} = C y^{3} + D y $ as $ h_{3} $ odd function. Letting $ h_{1}(y) = a_{1} y $ for some constant $ a_{1} $ we have:

\begin{align*}
0 & = (\psi_{1},\psi_{3}) \\
& = \int_{- \infty}^{\infty} \psi_{1}^{*} \psi_{3} \; \d y  \\
& = \int_{- \infty}^{\infty} a_{1} y \left( Cy^{3} + D y \right)e^{- y^{2} / 2}    \; \d y \\
& = a_{1} \left( 3 C   \sqrt{2 \pi} + B \sqrt{2 \pi}  \right) 
\end{align*}


Thus $ B = - 3 C $, and we can write $ \psi_{3}(x) = a_{3}(  y^{3} - 3 y ) $. 

Next, if the initial state can be written as $ \Psi(x,0) = \sum_{n=0}^{\infty} c_{n} \psi_{n}(x)  $, then

\begin{align*}
\Psi(x,t) & = \sum_{n=0}^{\infty} c_{n} \psi_{n}(x) e^{-iE_{n}t / \hbar} \\
& = \sum_{n=0}^{\infty} c_{n} \psi_{n}(x) e^{-i(n + \frac{1}{2}) \omega t} \\
& = 
\end{align*}



\section{QUESTION 5}

SE is

\[ - \frac{\hbar^{2}}{2m} \psi''(x) + V(x) \psi(x) = E \psi(x) \]

Probability current given by

\[ J(x) = - \frac{i \hbar }{2m} (\psi^{*} \psi' - (\psi^{*})' \psi )  \]

Differentiating with respect to $ x $,

\begin{align*}
\frac{\d J}{\d x}  & = - \frac{i \hbar }{2m}\left[ (\psi^{*})'\psi' + \psi^{*} \psi'' - (\psi^{*})'' \psi - (\psi^{*})' \psi'  \right]     \\
& =  - \frac{i \hbar }{2m}\left[ \psi^{*} \psi'' - (\psi^{*})'' \psi \right]     \\
& = - \frac{i \hbar }{2m}\left[ \psi^{*} \left(  - \frac{2m}{\hbar^{2}}(E - V) \psi \right)  - \left(  - \frac{2m}{\hbar^{2}}(E - V) \psi^{*} \right) \psi \right] \\
& = 0
\end{align*}

Probability current as $ x \to - \infty $, $ \psi(x) \sim e^{ikx} + Be^{-ikx} $ given by:

\begin{align*}
J & = - \frac{i \hbar }{2m} \left[   ( e^{-ikx} + B^{*} e^{ikx} )(ik e^{ikx} - i k B e^{-ikx}  )       - ( - i k e^{-i k x} + i k B^{*} e^{ikx}    )   ( e^{ikx} + Be^{-ikx}) \right] \\
& = - \frac{i \hbar }{2m} \left[  ik - ikBe^{-2ikx} + ikB^{*} e^{2ikx} - i k | B |^{2}  - \left(  - ik - ik B e^{-2ikx} + i k B^{*} e^{2ikx} + i k | B |^{2}     \right)    \right] \\
& = - \frac{i \hbar }{2m} \left[  2ik  - 2i k | B |^{2}    \right] \\
& =  \frac{\hbar k}{m} ( 1  - | B |^{2} )
\end{align*}

Probability current as $ x \to \infty $, $ \psi(x) C e^{ikx} $ given by:

\begin{align*}
J & = - \frac{i \hbar }{2m} \left[   (C^{*} e^{-ikx}  )(ik C e^{ikx}  )   - ( - i k C^{*} e^{-i k x})(C e^{ikx})  \right] \\
& = - \frac{i \hbar }{2m} \left[ 2ik | C |^{2}  \right] \\
& = \frac{\hbar k}{m} | C |^{2} 
\end{align*}

As independent of $ x $ these two expressions are equal, thus $ | B |^{2} + | C |^{2} = 1 $





\section{QUESTION 6}

Take the potential to be 

\begin{center}
	\begin{tikzpicture}
	\draw [->] (-3, 0) -- (5.5, 0) node [right] {$x$};
	\draw [->] (2, 0) -- (2, 3) node [above] {$V$};
	\node [left] at (2, 2) {$U$};
	\node [below] at (2, 0) {$0$};
	
	\node [below] at (3, 0) {$a$};
	\draw [mred, semithick] (-3, 0) -- (2, 0) -- (2, 2) -- (3, 2) -- (3, 0) -- (5, 0);
	\end{tikzpicture}
\end{center}

\[ V(x) = \begin{cases} U  & \text{ if } 0 < x < a \\ 0  & \text{ othewise } \end{cases} \]

where $ U = 2E $. Set the constant

\[
E = \frac{\hbar^2 k^2}{2m}
\]

Then the Schr\"odinger equations become
\begin{align*}
\psi'' + k^2 \psi &= 0 && x < 0\\
\psi'' - k^2 \psi &= 0 && 0 < x < a\\
\psi'' + k^2 \psi &= 0 && x > a
\end{align*}
So we get
\begin{align*}
\psi &= I e^{ikx} + Re^{-ikx}&& x < 0\\
\psi &= Ae^{k x} + Be^{-k x}&& 0 < x < a\\
\psi &= Te^{ikx} && x > a
\end{align*}
(no $ e^{-ikx} $ term $ \iff $ no particles sent from right)

Matching $\psi$ and $\psi'$ at $x = 0$ and $a$ gives the equations
\begin{align*}
I + R &= A + B\\
ik(I - R) &= k (A - B)\\
A e^{k a} + Be^{- k a} &= Te^{ika}\\
k(Ae^{k a} - Be^{k a}) &= ik Te^{ika}.
\end{align*}
We can solve these to obtain
\begin{align*}
I + \frac{k - ik}{k + ik}R &= Te^{ika} e^{-k a}\\
I + \frac{k + ik}{k - ik}R &= Te^{ika} e^{k a}.
\end{align*}
After \st{lots of} \emph{some} algebra, we obtain
\begin{align*}
T &= I e^{-ika}\left(\cosh k a\right)^{-1}
\end{align*}
To interpret this, we use the currents
\[
j = j_{\mathrm{inc}} + j_{\mathrm{ref}} = (|I|^2 - |R|^2) \frac{\hbar k}{m}
\]
for $x < 0$. On the other hand, we have
\[
j = j_{\mathrm{tr}} = |T|^2 \frac{\hbar k}{m}
\]
for $x > a$. We can use these to find the transmission probability, and it turns out to be
\[
P_{\mathrm{tr}} = \frac{|j_{\mathrm{tr}j}|}{|j_{\mathrm{inc}}|} = \frac{|T|^2}{|I|^2} = \left[ \cosh^{2} ka \right]^{-1}.
\]
This demonstrates \emph{quantum tunneling}. There is a non-zero probability that the particles can pass through the potential barrier even though it classically does not have enough energy.

\section{QUESTION 7}


Time independent SE is 

\[ - \frac{\hbar^{2}}{2m} \psi'' - U \delta(x) \psi = E \psi  \]




\section{QUESTION 8}

\begin{enumerate}
	\item \begin{align*}
	1 & = \int_{0}^{a} | \Psi |^{2} \; \d x  \\
	& = C^{2} \int_{0}^{a} x^{2} (a-x)^{2} \; \d x\\
	& = C^{2} \frac{a^{5}}{30} 
	\end{align*}
	
	So $ C = \sqrt{30 } a^{-5/2} $
	
	\item 
	
\end{enumerate}


\section{QUESTION 9}


$ Q \psi_{n} = 0 \; \forall \;  n > 2 \Rightarrow  $ zero is an eigenvalue. We are also given

\[ Q \psi_{1} = \psi_{2}, Q \psi_{2} = \psi_{1} \]

Adding (and using linearity) gives $ Q(\psi_{1} + \psi_{2})  = \psi_{1} + \psi_{2} $, thus $ 1 $ is an eigenvalue of $ Q $. Similarly subtracting shows that $ Q (\psi_{1} - \psi_{2}) = - (\psi_{1} - \psi_{2}) $, ie. $ -1 $ is an eigenvalue. 

To find normalised eigenstates, 

\begin{align*}
1 & = \int | C |^{2} | \psi_{1} + \psi_{2} |^{2} \; \d x  \\
& = | C^{2} | \int  (\psi_{1} + \psi_{2})^{*} ( \psi_{1} + \psi_{2}) \; \d x\\
& = |  C^{2} | \int | \psi_{1} |^{2} + | \psi_{2} |^{2} \qquad ( \text{by orthoganilty of eigenstates})\\
& = 2 | C^{2} | \quad \text{ as } \psi_{n} \text{ normalised}
\end{align*}

Thus $ \chi_{+} = \frac{1}{\sqrt{2}} (\psi_{1} + \psi_{2})  $, and similarly $ \chi_{-} = \frac{1}{\sqrt{2}} ( \psi_{1} - \psi_{2})  $


\begin{align*}
\langle H \rangle_{\chi_{\pm}} & = ( \chi_{\pm}, H \chi_{\pm} )  \\
& = \frac{1}{\sqrt{2}} (  (\psi_{1} \pm \psi_{2}),  H( \psi_{1} \pm \psi_{2} ) \\
& = \frac{1}{\sqrt{2}} (  (\psi_{1}, H \psi_{1}) \pm  ( \psi_{2}, H \psi_{2} ) \\
& = \frac{1}{\sqrt{2}} ( E_{1} \pm E_{2} )
\end{align*}

Measurement axioms $ \Rightarrow  $ at time zero, $ Q $ is in state $ \chi_{+} $. 
Have

\[ \Psi(0) = \alpha_{+} \chi_{+} + \alpha_{-} \chi_{-} \qquad (\alpha_{\pm} = (\chi_{\pm},\Psi(0) )) \]

By linearity, the solution of the t-dep SE is

\begin{align*}
\Psi(t) & = \alpha_{+} \chi_{+} e^{- i E_{+} t / \hbar } + \alpha_{-} \chi_{-} e^{- i E_{-} t / \hbar }  \\
& = 
\end{align*}



\section{QUESTION 10}


\begin{align*}
\langle [H,A] \rangle_{\psi} & = \langle HA - AH \rangle_{\psi}  \\
& = (  \psi, (HA - AH)\psi ) \\
& = ( \psi, HA \psi) - ( \psi, AH \psi) \\
& = ( H \psi, A \psi) - ( \psi, AH \psi)
\end{align*}

\section{QUESTION 11}






\end{document}